examples/Messaging/Election.v
@@ -1,0 +1,74 @@
+From ITree Require Import
+     Subevent
+     CategoryOps
+     Indexed.Sum.
+
+From Coq Require Import Nat List.
+
+From Coq Require Import
+     Vector
+     List
+     Arith.PeanoNat.
+
+From ITree Require Import
+     CategoryOps.
+
+From ExtLib Require Import
+     Structures.MonadState
+     Data.Monads.StateMonad.
+
+From CTree Require Import
+     CTree
+     Eq
+     Interp.Preempt
+     Interp.Network
+     Logic.Kripke
+     Logic.Ctl.
+
+Import CTreeNotations ListNotations VectorNotations CtlNotations.
+Local Open Scope vector_scope.
+Local Open Scope ctree_scope.
+Local Open Scope ctl_scope.
+
+Set Implicit Arguments.
+
+Variant csE: Type -> Type :=
+  | In_CS: bool -> csE unit.
+
+Definition enter_cs {E C} `{csE -< E}: ctree E C unit :=
+  trigger (In_CS true). 
+Definition exit_cs {E C} `{csE -< E}: ctree E C unit :=
+  trigger (In_CS false). 
+
+#[global] Instance handler_cs: csE ~~> state bool :=
+  fun _ e => match e with In_CS b => put b end.
+
+(*| Client process |*)
+Definition proc (id: uid)(n: nat): ctree ((netE uid +' parE) +' csE) B01 unit :=
+  let right := modulo (S id) n in
+  CTree.forever (fun _ =>
+      (* 1. Send my [id] to the process on the right *)
+      send right id;;
+      (* 2. Loop until received [CS] message *)
+      CTree.iter (fun _ =>
+                    m <- recv;;
+                    match m with
+                    | Some x =>
+                        match Nat.compare x id with
+                        (* Maybe my [right] neighbor is the leader *)
+                        | Gt => send right x;; Ret (inr tt)
+                        (* smaller [id] means definitely not the leader *)
+                        | Lt => Ret (inr tt)
+                        (* I am the leader! *)
+                        | Eq => enter_cs ;; Ret (inr tt)
+                        end                    
+                    | None => Ret (inl tt)
+                    end) tt) tt.
+
+Lemma election_live: 
+    <( {rr [proc 0 3; proc 1 3; proc 2 3]},
+     {([]%list, 0, false)} |= AG (AF now {fun '(_, b) => b = true}) )>.
+Proof.
+  unfold rr.
+  eapply ctl_forever_ar.
+Admitted.  
